hol/cake_sem/p4_cake_transformScript.sml
@@ -396,20 +396,36 @@ Definition transform_v_def:
   | v_bot => SOME $ v'_bot)
 End
 
+(* Note this only permits matching with up to 128 bits *)
 Definition transform_s_def:
  transform_s dict s =
   case s of
    s_sing v =>
   (case v of
-   | v_bit (bl, n) => SOME (s'_sing $ v2w bl, n)
+   | v_bit (bl, n) =>
+    if n <= 128
+    then if n <= 64
+    then SOME (s'_sing $ (0w, v2w bl), n)
+    else SOME (s'_sing $ (v2w $ TAKE (n-64) bl, v2w $ DROP (n-64) bl), n)
+    else NONE
    | _ => NONE)
  | s_range (bl1, n1) (bl2, n2) =>
-  if n1 <= 64 /\ n2 <= 64
-  then SOME (s'_range (v2w bl1) (v2w bl2), n1)
+  if n1 <= 128 /\ n2 <= 128
+  then
+   let w'1 = if n1 <= 64 then 0w else v2w $ TAKE (n1-64) bl1 in
+   let w'2 = if n1 <= 64 then v2w bl1 else v2w $ DROP (n1-64) bl1 in
+   let w''1 = if n2 <= 64 then 0w else v2w $ TAKE (n2-64) bl2 in
+   let w''2 = if n2 <= 64 then v2w bl2 else v2w $ DROP (n2-64) bl2 in
+    SOME (s'_range (w'1, w'2) (w''1, w''2), n1)
   else NONE
  | s_mask (bl1, n1) (bl2, n2) =>
-  if n1 <= 64 /\ n2 <= 64
-  then SOME (s'_mask (v2w bl1) (v2w bl2), n1)
+  if n1 <= 128 /\ n2 <= 128
+  then
+   let w'1 = if n1 <= 64 then 0w else v2w $ TAKE (n1-64) bl1 in
+   let w'2 = if n1 <= 64 then v2w bl1 else v2w $ DROP (n1-64) bl1 in
+   let w''1 = if n2 <= 64 then 0w else v2w $ TAKE (n2-64) bl2 in
+   let w''2 = if n2 <= 64 then v2w bl2 else v2w $ DROP (n2-64) bl2 in
+    SOME (s'_mask (w'1, w'2) (w''1, w''2), n1)
   else NONE
  | s_univ => SOME (s'_univ, 0)
 End
